Checkpoint

LinearScan/Lib.hs
@@ -326,3 +326,49 @@ list_membership a l =
    (:) x xs -> (:) x
     ((Prelude.map) (exist_in_cons a x xs) (list_membership a xs))}
 
+imerge :: (a1 -> Prelude.Int) -> ([] a1) -> ([] a1) -> [] a1
+imerge f l1 l2 =
+  let {
+   imerge_aux l3 =
+     case l1 of {
+      [] -> l3;
+      (:) a1 l1' ->
+       case l3 of {
+        [] -> l1;
+        (:) a2 l2' ->
+         case (Prelude.<=) (f a1) (f a2) of {
+          Prelude.True -> (:) a1 (imerge f l1' l3);
+          Prelude.False -> (:) a2 (imerge_aux l2')}}}}
+  in imerge_aux l2
+
+imerge_list_to_stack :: (a1 -> Prelude.Int) -> ([] (Prelude.Maybe ([] a1)))
+                        -> ([] a1) -> [] (Prelude.Maybe ([] a1))
+imerge_list_to_stack f stack l =
+  case stack of {
+   [] -> (:) (Prelude.Just l) [];
+   (:) y stack' ->
+    case y of {
+     Prelude.Just l' -> (:) Prelude.Nothing
+      (imerge_list_to_stack f stack' (imerge f l' l));
+     Prelude.Nothing -> (:) (Prelude.Just l) stack'}}
+
+imerge_stack :: (a1 -> Prelude.Int) -> ([] (Prelude.Maybe ([] a1))) -> [] a1
+imerge_stack f stack =
+  case stack of {
+   [] -> [];
+   (:) y stack' ->
+    case y of {
+     Prelude.Just l -> imerge f l (imerge_stack f stack');
+     Prelude.Nothing -> imerge_stack f stack'}}
+
+iter_imerge :: (a1 -> Prelude.Int) -> ([] (Prelude.Maybe ([] a1))) -> ([] 
+               a1) -> [] a1
+iter_imerge f stack l =
+  case l of {
+   [] -> imerge_stack f stack;
+   (:) a l' -> iter_imerge f (imerge_list_to_stack f stack ((:) a [])) l'}
+
+isort :: (a1 -> Prelude.Int) -> ([] a1) -> [] a1
+isort f =
+  iter_imerge f []
+
